Weidenbach_Book/IsaSAT_Clauses.thy
@@ -1,5 +1,5 @@
 theory IsaSAT_Clauses
-imports Watched_Literals.Watched_Literals_Watch_List_Code_Common IsaSAT_Arena
+imports IsaSAT_Arena
 begin
 
 (* TODO This file should probably be merged with IsaSAT_Arena*)
@@ -42,7 +42,7 @@ definition fmap_rll :: "(nat, 'a literal list \<times> bool) fmap \<Rightarrow> 
 
 definition fmap_rll_u :: "(nat, 'a literal list \<times> bool) fmap \<Rightarrow> nat \<Rightarrow> nat \<Rightarrow> 'a literal" where
   [simp]: \<open>fmap_rll_u  = fmap_rll\<close>
-(* 
+(*
 lemma nth_clauses_rll:
   \<open>(uncurry2 (RETURN ooo (\<lambda>(N, _) i. Array_List_Array.nth_rll N i)), uncurry2 (RETURN ooo IsaSAT_Clauses.fmap_rll))
     \<in> [\<lambda>((N, i), j). i \<in># dom_m N \<and> j < length (N \<propto> i)]\<^sub>f
@@ -255,87 +255,6 @@ definition fmap_length_rll_u64 :: "(nat, 'a literal list \<times> bool) fmap \<R
 
 declare fmap_length_rll_u_def[symmetric, isasat_codegen]
 
-definition length_raa_u32_u64 :: \<open>'a::heap arrayO_raa \<Rightarrow> uint32 \<Rightarrow> uint64 Heap\<close> where
-  \<open>length_raa_u32_u64 xs i = do {
-     x \<leftarrow> arl_get_u xs i;
-    length_u64_code x}\<close>
-
-lemma length_raa_u32_u64_hnr[sepref_fr_rules]:
-  shows \<open>(uncurry length_raa_u32_u64, uncurry (RETURN \<circ>\<circ> length_rll_n_uint64)) \<in>
-     [\<lambda>(xs, i). i < length xs \<and> length (xs ! i) \<le> uint64_max]\<^sub>a
-       (arlO_assn (array_assn R))\<^sup>k *\<^sub>a uint32_nat_assn\<^sup>k \<rightarrow> uint64_nat_assn\<close>
-proof -
-   have 1: \<open>a * b * c = c * a * b\<close> for a b c :: assn
-    by (auto simp: ac_simps)
-  have H: \<open><arlO_assn_except (array_assn R) [nat_of_uint32 bi] a (aa, ba)
-        (\<lambda>r'. array_assn R (a ! nat_of_uint32 bi) x *
-              \<up> (x = r' ! nat_of_uint32 bi))>
-      Array.len x <\<lambda>r. \<up>(r = length (a ! nat_of_uint32 bi)) *
-          arlO_assn (array_assn R) a (aa, ba)>\<close>
-    if
-      \<open>nat_of_uint32 bi < length a\<close> and
-      \<open>length (a ! nat_of_uint32 bi) \<le> uint64_max\<close>
-    for bi :: \<open>uint32\<close> and a :: \<open>'b list list\<close> and aa :: \<open>'a array array\<close> and ba :: \<open>nat\<close> and
-      x :: \<open>'a array\<close>
-  proof -
-    show ?thesis
-      using that apply -
-      apply (subst arlO_assn_except_array0_index[symmetric, OF that(1)])
-      by (sep_auto simp: array_assn_def arl_get_def hr_comp_def is_array_def
-          list_rel_imp_same_length arlO_assn_except_def)
-  qed
-  show ?thesis
-  apply sepref_to_hoare
-  apply (sep_auto simp: uint64_nat_rel_def br_def length_rll_def
-      nat_of_uint64_uint64_of_nat_id length_raa_u32_u64_def arl_get_u_def arl_get'_def
-      uint32_nat_rel_def nat_of_uint32_code[symmetric] length_u64_code_def
-      intro!:)+
-     apply (rule H; assumption)
-    apply (sep_auto simp: array_assn_def arl_get_def nat_of_uint64_uint64_of_nat_id)
-    done
-qed
-
-
-definition length_raa_u64_u64 :: \<open>'a::heap arrayO_raa \<Rightarrow> uint64 \<Rightarrow> uint64 Heap\<close> where
-  \<open>length_raa_u64_u64 xs i = do {
-     x \<leftarrow> arl_get_u64 xs i;
-    length_u64_code x}\<close>
-
-lemma length_raa_u64_u64_hnr[sepref_fr_rules]:
-  shows \<open>(uncurry length_raa_u64_u64, uncurry (RETURN \<circ>\<circ> length_rll_n_uint64)) \<in>
-     [\<lambda>(xs, i). i < length xs \<and> length (xs ! i) \<le> uint64_max]\<^sub>a
-       (arlO_assn (array_assn R))\<^sup>k *\<^sub>a uint64_nat_assn\<^sup>k \<rightarrow> uint64_nat_assn\<close>
-proof -
-   have 1: \<open>a * b * c = c * a * b\<close> for a b c :: assn
-    by (auto simp: ac_simps)
-  have H: \<open><arlO_assn_except (array_assn R) [nat_of_uint64 bi] a (aa, ba)
-        (\<lambda>r'. array_assn R (a ! nat_of_uint64 bi) x *
-              \<up> (x = r' ! nat_of_uint64 bi))>
-      Array.len x <\<lambda>r. \<up>(r = length (a ! nat_of_uint64 bi)) *
-          arlO_assn (array_assn R) a (aa, ba)>\<close>
-    if
-      \<open>nat_of_uint64 bi < length a\<close> and
-      \<open>length (a ! nat_of_uint64 bi) \<le> uint64_max\<close>
-    for bi :: \<open>uint64\<close> and a :: \<open>'b list list\<close> and aa :: \<open>'a array array\<close> and ba :: \<open>nat\<close> and
-      x :: \<open>'a array\<close>
-  proof -
-    show ?thesis
-      using that apply -
-      apply (subst arlO_assn_except_array0_index[symmetric, OF that(1)])
-      by (sep_auto simp: array_assn_def arl_get_def hr_comp_def is_array_def
-          list_rel_imp_same_length arlO_assn_except_def)
-  qed
-  show ?thesis
-  apply sepref_to_hoare
-  apply (sep_auto simp: uint64_nat_rel_def br_def length_rll_def
-      nat_of_uint64_uint64_of_nat_id length_raa_u32_u64_def arl_get_u64_def arl_get'_def
-      uint32_nat_rel_def nat_of_uint32_code[symmetric] length_u64_code_def length_raa_u64_u64_def
-      nat_of_uint64_code[symmetric]
-      intro!:)+
-     apply (rule H; assumption)
-    apply (sep_auto simp: array_assn_def arl_get_def nat_of_uint64_uint64_of_nat_id)
-    done
-qed
 
 sepref_definition length_raa_u64_clss
   is \<open>uncurry ((RETURN \<circ>\<circ>\<circ> case_prod) (\<lambda>N _. length_rll_n_uint64 N))\<close>
@@ -443,37 +362,6 @@ definition fmap_length_rll :: "(nat, 'a literal list \<times> bool) fmap \<Right
     \<in> [\<lambda>(N, i). i \<in># dom_m N]\<^sub>f \<langle>Id\<rangle>clauses_l_fmat \<times>\<^sub>r nat_rel \<rightarrow> \<langle>nat_rel\<rangle>nres_rel\<close>
   by (intro frefI nres_relI) (auto simp: list_fmap_rel_def fmap_length_rll_def length_rll_def) *)
 
-
-definition length_raa_u32 :: \<open>'a::heap arrayO_raa \<Rightarrow> uint32 \<Rightarrow> nat Heap\<close> where
-  \<open>length_raa_u32 xs i = do {
-     x \<leftarrow> arl_get_u xs i;
-    Array.len x}\<close>
-
-lemma length_raa_u32_rule[sep_heap_rules]:
-  \<open>b < length xs \<Longrightarrow> (b', b) \<in> uint32_nat_rel \<Longrightarrow> <arlO_assn (array_assn R) xs a> length_raa_u32 a b'
-   <\<lambda>r. arlO_assn (array_assn R) xs a * \<up> (r = length_rll xs b)>\<^sub>t\<close>
-  supply arrayO_raa_nth_rule[sep_heap_rules]
-  unfolding length_raa_u32_def arl_get_u_def arl_get'_def uint32_nat_rel_def br_def
-  apply (cases a)
-  apply (sep_auto simp: nat_of_uint32_code[symmetric])
-  apply (sep_auto simp: arlO_assn_except_def arl_length_def array_assn_def
-      eq_commute[of \<open>(_, _)\<close>] is_array_def hr_comp_def length_rll_def
-      dest: list_all2_lengthD)
-   apply (sep_auto simp: arlO_assn_except_def arl_length_def arl_assn_def
-      hr_comp_def[abs_def] arl_get'_def
-      eq_commute[of \<open>(_, _)\<close>] is_array_list_def hr_comp_def length_rll_def list_rel_def
-      dest: list_all2_lengthD)[]
-  unfolding arlO_assn_def[symmetric] arl_assn_def[symmetric]
-  apply (subst arlO_assn_except_array0_index[symmetric, of b])
-   apply simp
-  unfolding arlO_assn_except_def arl_assn_def hr_comp_def is_array_def
-  apply sep_auto
-  done
-
-lemma length_raa_u32_hnr[sepref_fr_rules]:
-  \<open>(uncurry length_raa_u32, uncurry (RETURN \<circ>\<circ> length_rll)) \<in>
-     [\<lambda>(xs, i). i < length xs]\<^sub>a (arlO_assn (array_assn R))\<^sup>k *\<^sub>a uint32_nat_assn\<^sup>k \<rightarrow> nat_assn\<close>
-  by sepref_to_hoare sep_auto
 
 
 sepref_definition length_raa_u32_clss
@@ -643,47 +531,6 @@ definition fm_add_new_at_position
 where
   \<open>fm_add_new_at_position b i C N = fmupd i (C, b) N\<close>
 
-(* definition append_and_length
-   :: \<open>bool \<Rightarrow> 'v clause_l \<Rightarrow> 'v clause_l list \<times> clause_annots \<Rightarrow> ('v clause_l list \<times> clause_annots) \<times> nat\<close>
-where
-\<open>append_and_length b C = (\<lambda>(N, cs).
-     let k = length N in
-     let b' = (if b then IRRED else LEARNED, 0, 0) in
-       ((op_list_append N C, op_list_append cs b'), k))\<close> *)
-(* 
-lemma append_and_length_fm_add_new:
-  \<open>(uncurry2 (RETURN ooo append_and_length), uncurry2 fm_add_new)
-     \<in> bool_rel \<times>\<^sub>f (\<langle>Id\<rangle>list_rel) \<times>\<^sub>f (clauses_l_fmat) \<rightarrow>\<^sub>f \<langle>clauses_l_fmat \<times>\<^sub>f nat_rel\<rangle>nres_rel\<close>
-  apply (intro frefI nres_relI)
-  apply (auto simp: fm_add_new_at_position_def list_fmap_rel_def Let_def
-      max_def nth_append append_and_length_def fm_add_new_def get_fresh_index_def
-      RETURN_RES_refine_iff RES_RETURN_RES
-      intro!: RETURN_SPEC_refine
-      dest: multi_member_split
-      split: if_splits)
-  apply force
-  apply force
-  apply force
-   apply force
-   apply force
-  apply (case_tac \<open>set_mset (dom_m bc) = {}\<close>)
-  apply force
-  apply force
-  apply (case_tac \<open>set_mset (dom_m bc) = {}\<close>)
-  apply force
-   apply force
-  apply (case_tac \<open>set_mset (dom_m bc) = {}\<close>)
-   apply force
-  apply (subst extra_clause_information_upd_irrel)
-    apply force
-  apply auto
-  apply (case_tac \<open>set_mset (dom_m bc) = {}\<close>)
-   apply force
-    apply force
-  apply (subst extra_clause_information_upd_irrel)
-  apply auto
-  done *)
-
 definition AStatus_IRRED where
   \<open>AStatus_IRRED = AStatus IRRED\<close>
 
@@ -740,38 +587,6 @@ lemma ALit_hnr[sepref_fr_rules]:
 
 declare is_short_clause_code.refine[sepref_fr_rules]
 
-
-lemma le_uint32_max_le_uint64_max: \<open>a \<le> uint32_max + 2 \<Longrightarrow> a \<le> uint64_max\<close>
-  by (auto simp: uint32_max_def uint64_max_def)
-
-lemma nat_of_uint64_ge_minus:
-  \<open>ai >= bi \<Longrightarrow>
-       nat_of_uint64 (ai - bi) = nat_of_uint64 ai - nat_of_uint64 bi\<close>
-  apply transfer
-  unfolding unat_def
-  by (subst uint_sub_lem[THEN iffD1])
-    (auto simp: unat_def uint_nonnegative nat_diff_distrib word_le_def[symmetric] intro: leI)
-
-lemma minus_uint64_nat_assn[sepref_fr_rules]:
-  \<open>(uncurry (return oo (-)), uncurry (RETURN oo (-))) \<in> 
-    [\<lambda>(a, b). a \<ge> b]\<^sub>a uint64_nat_assn\<^sup>k *\<^sub>a uint64_nat_assn\<^sup>k \<rightarrow> uint64_nat_assn\<close>
-  by sepref_to_hoare
-    (sep_auto simp: uint64_nat_rel_def br_def nat_of_uint64_ge_minus
-   nat_of_uint64_le_iff)
-
-definition uint32_of_uint64 where
-  \<open>uint32_of_uint64 n = uint32_of_nat (nat_of_uint64 n)\<close>
-
-definition uint32_of_uint64_rel where
-  [simp]: \<open>uint32_of_uint64_rel n = n\<close>
-
-lemma uint32_of_uint64_rel_hnr[sepref_fr_rules]:
-  \<open>(return o uint32_of_uint64, RETURN o uint32_of_uint64_rel) \<in>
-     [\<lambda>a. a \<le> uint32_max]\<^sub>a uint64_nat_assn\<^sup>k \<rightarrow> uint32_nat_assn\<close>
-  by sepref_to_hoare
-    (sep_auto simp: uint32_of_uint64_def uint32_nat_rel_def br_def nat_of_uint64_le_iff
-      nat_of_uint32_uint32_of_nat_id uint64_nat_rel_def)
-
 sepref_definition header_size_code
   is \<open>RETURN o header_size\<close>
   :: \<open>clause_ll_assn\<^sup>k \<rightarrow>\<^sub>a nat_assn\<close>
@@ -789,25 +604,25 @@ sepref_definition append_and_length_code
    AStatus_LEARNED_def[symmetric]
    two_uint64_nat_def[symmetric]
    apply (rewrite in \<open>let _ = _ - _ in _\<close> length_uint64_nat_def[symmetric])
-   apply (rewrite in \<open>let _ = _ in let _ = _ in let _ = \<hole> in _\<close> uint32_of_uint64_rel_def[symmetric])
+   apply (rewrite in \<open>let _ = _ in let _ = _ in let _ = \<hole> in _\<close> uint32_of_uint64_conv_def[symmetric])
    apply (rewrite in \<open>_ < length _\<close> length_uint64_nat_def[symmetric])
   by sepref
 
 declare append_and_length_code.refine[sepref_fr_rules]
 
-(* 
+(*
 lemma fm_add_new_hnr[sepref_fr_rules]:
   \<open>(uncurry2 append_and_length_code, uncurry2 fm_add_new)
     \<in> bool_assn\<^sup>k *\<^sub>a clause_ll_assn\<^sup>d *\<^sub>a clauses_ll_assn\<^sup>d \<rightarrow>\<^sub>a clauses_ll_assn *a nat_assn\<close>
   using append_and_length_code.refine[FCOMP append_and_length_fm_add_new]
   unfolding clauses_ll_assn_def by simp *)
 
-(* 
+(*
 definition get_fresh_index_packed :: \<open>'v clauses_l \<Rightarrow> nat nres\<close> where
 \<open>get_fresh_index_packed N = SPEC(\<lambda>i. i > 0 \<and> i \<notin># dom_m N \<and>
     (\<forall>j < i. j > 0 \<longrightarrow> j \<in># dom_m N))\<close>
 
-lemma (in -)get_fresh_index_packed_alt_def: 
+lemma (in -)get_fresh_index_packed_alt_def:
   assumes \<open>packed N\<close>
   shows \<open>get_fresh_index_packed N = SPEC (\<lambda>i. i = Suc (Max_dom N))\<close>
 proof -
@@ -842,7 +657,7 @@ definition fm_add_new_packed where
       Max_dom_alt_def[symmetric] Max_dom_fmupd_irrel
       intro!: RETURN_SPEC_refine
       intro: packed_in_dom_mI) *)
-(* 
+(*
 lemma fm_add_new_packed_hnr[sepref_fr_rules]:
   \<open>(uncurry2 append_and_length_code, uncurry2 fm_add_new_packed)
     \<in> [\<lambda>(_, N). packed N]\<^sub>a bool_assn\<^sup>k *\<^sub>a clause_ll_assn\<^sup>d *\<^sub>a clauses_ll_assn\<^sup>d \<rightarrow> clauses_ll_assn *a nat_assn\<close>
@@ -850,47 +665,12 @@ lemma fm_add_new_packed_hnr[sepref_fr_rules]:
   unfolding clauses_ll_assn_def
   by simp *)
 
-(* TODO Proper setup + Move *)
-definition length_arlO_u where
-  \<open>length_arlO_u xs = do {
-      n \<leftarrow> length_ra xs;
-      return (uint32_of_nat n)}\<close>
-
-lemma length_arlO_u[sepref_fr_rules]:
-  \<open>(length_arlO_u, RETURN o length_u) \<in> [\<lambda>xs. length xs \<le> uint32_max]\<^sub>a (arlO_assn R)\<^sup>k \<rightarrow> uint32_nat_assn\<close>
-  by sepref_to_hoare
-    (sep_auto simp: length_arlO_u_def arl_length_def uint32_nat_rel_def
-      br_def nat_of_uint32_uint32_of_nat_id)
-
-definition arl_length_u64_code where
-\<open>arl_length_u64_code C = do {
-  n \<leftarrow> arl_length C;
-  return (uint64_of_nat n)
-}\<close>
-
-lemma arl_length_u64_code[sepref_fr_rules]:
-  \<open>(arl_length_u64_code, RETURN o length_uint64_nat) \<in>
-     [\<lambda>xs. length xs \<le> uint64_max]\<^sub>a (arl_assn R)\<^sup>k \<rightarrow> uint64_nat_assn\<close>
-  by sepref_to_hoare
-    (sep_auto simp: arl_length_u64_code_def arl_length_def uint64_nat_rel_def
-      br_def nat_of_uint64_uint64_of_nat_id arl_assn_def hr_comp_def[abs_def]
-      is_array_list_def dest: list_rel_imp_same_length)
-(* End Move *)
-
-definition convert_to_uint32 :: \<open>nat \<Rightarrow> nat\<close> where
-  [simp]: \<open>convert_to_uint32 = id\<close>
-
-lemma convert_to_uint32_hnr[sepref_fr_rules]:
-  \<open>(return o uint32_of_nat, RETURN o convert_to_uint32)
-    \<in> [\<lambda>n. n \<le> uint32_max]\<^sub>a nat_assn\<^sup>k \<rightarrow> uint32_nat_assn\<close>
-  by sepref_to_hoare
-    (sep_auto simp: uint32_nat_rel_def br_def uint32_max_def nat_of_uint32_uint32_of_nat_id)
 
 lemma fm_add_new_alt_def:
  \<open>fm_add_new b C N = do {
       let st = (if b then AStatus_IRRED else AStatus_LEARNED);
       let l = length_uint64_nat N;
-      let s = uint32_of_uint64_rel (length_uint64_nat C - two_uint64_nat);
+      let s = uint32_of_uint64_conv (length_uint64_nat C - two_uint64_nat);
       let N =
         (if is_short_clause C
           then (((N @ [st]) @ [AActivity zero_uint32_nat]) @ [ALBD s]) @
@@ -913,15 +693,15 @@ lemma fm_add_new_alt_def:
 
 definition fm_add_new_fast where
   [simp, symmetric]: \<open>fm_add_new_fast = fm_add_new\<close>
-(* 
+(*
 lemma fm_add_new_fast_hnr[sepref_fr_rules]:
   \<open>(uncurry2 append_and_length_u32_code, uncurry2 fm_add_new_fast)
     \<in> [\<lambda>((b, C), N). length C \<le> uint32_max+1 \<and> length C \<ge> 2 \<and>
-        length N \<le> uint64_max]\<^sub>a 
+        length N \<le> uint64_max]\<^sub>a
        bool_assn\<^sup>k *\<^sub>a clause_ll_assn\<^sup>d *\<^sub>a arena_assn\<^sup>d \<rightarrow> arena_assn *a uint64_nat_assn\<close>
   using append_and_length_u32_code.refine by simp *)
 
-(* 
+(*
 lemma append_and_length_u32_fm_add_new_packed:
   \<open>(uncurry2 append_and_length_u32, uncurry2 fm_add_new_packed)
      \<in> [\<lambda>((b, C), N). Max (insert 0 (set_mset (dom_m N))) < uint32_max \<and> packed N]\<^sub>f
@@ -942,7 +722,7 @@ lemma append_and_length_u32_fm_add_new_packed:
       intro: packed_in_dom_mI
       split: if_splits)
   done *)
-(* 
+(*
 definition fm_add_new_packed_fast where
   [simp, symmetric]: \<open>fm_add_new_packed_fast = fm_add_new_packed\<close>
 
