Weidenbach_Book/IsaSAT_Literals.thy
@@ -1,7 +1,574 @@
-theory Watched_Literals_Watch_List_Code_Common
-  imports Watched_Literals_Watch_List_Domain
-     Bits_Natural WB_Word_Assn
+theory IsaSAT_Literals
+  imports Watched_Literals.Watched_Literals_Watch_List_Domain
+     Watched_Literals.Bits_Natural Watched_Literals.WB_Word_Assn
 begin
+
+
+subsubsection \<open>Refinement of the Watched Function\<close>
+
+definition map_fun_rel :: \<open>(nat \<times> 'key) set \<Rightarrow> ('b \<times> 'a) set \<Rightarrow> ('b list \<times> ('key \<Rightarrow> 'a)) set\<close> where
+  map_fun_rel_def_internal:
+    \<open>map_fun_rel D R = {(m, f). \<forall>(i, j)\<in>D. i < length m \<and> (m ! i, f j) \<in> R}\<close>
+
+lemma map_fun_rel_def:
+  \<open>\<langle>R\<rangle>map_fun_rel D = {(m, f). \<forall>(i, j)\<in>D. i < length m \<and> (m ! i, f j) \<in> R}\<close>
+  unfolding relAPP_def map_fun_rel_def_internal by auto
+
+definition map_fun_rel_assn
+   :: \<open>(nat \<times> nat literal) set \<Rightarrow> ('a \<Rightarrow> 'b \<Rightarrow> assn) \<Rightarrow> (nat literal \<Rightarrow> 'a) \<Rightarrow> 'b list \<Rightarrow> assn\<close>
+where
+  \<open>map_fun_rel_assn D R = pure (\<langle>the_pure R\<rangle>map_fun_rel D)\<close>
+
+lemma [safe_constraint_rules]: \<open>is_pure (map_fun_rel_assn D R)\<close>
+  unfolding map_fun_rel_assn_def by auto
+
+
+subsection \<open>Literals as Natural Numbers\<close>
+
+subsubsection \<open>Definition\<close>
+
+lemma Pos_div2_iff:
+   \<open>Pos ((bb :: nat) div 2) = b \<longleftrightarrow> is_pos b \<and> (bb = 2 * atm_of b \<or> bb = 2 * atm_of b + 1)\<close>
+  by (cases b) auto
+lemma Neg_div2_iff:
+   \<open>Neg ((bb :: nat) div 2) = b \<longleftrightarrow> is_neg b \<and> (bb = 2 * atm_of b \<or> bb = 2 * atm_of b + 1)\<close>
+  by (cases b) auto
+
+text \<open>
+  Modeling \<^typ>\<open>nat literal\<close> via the transformation associating \<^term>\<open>2*n\<close> or \<^term>\<open>2*n+1\<close>
+  has some advantages over the transformation to positive or negative integers: 0 is not an issue.\<close>
+fun nat_of_lit :: \<open>nat literal \<Rightarrow> nat\<close> where
+  \<open>nat_of_lit (Pos L) = 2*L\<close>
+| \<open>nat_of_lit (Neg L) = 2*L + 1\<close>
+
+lemma nat_of_lit_def: \<open>nat_of_lit L = (if is_pos L then 2 * atm_of L else 2 * atm_of L + 1)\<close>
+  by (cases L) auto
+
+fun literal_of_nat :: \<open>nat \<Rightarrow> nat literal\<close> where
+  \<open>literal_of_nat n = (if even n then Pos (n div 2) else Neg (n div 2))\<close>
+
+lemma lit_of_nat_nat_of_lit[simp]: \<open>literal_of_nat (nat_of_lit L) = L\<close>
+  by (cases L) auto
+
+lemma nat_of_lit_lit_of_nat[simp]: \<open>nat_of_lit (literal_of_nat n) = n\<close>
+  by auto
+
+lemma atm_of_lit_of_nat: \<open>atm_of (literal_of_nat n) = n div 2\<close>
+  by auto
+
+text \<open>There is probably a more ``closed'' form from the following theorem, but it is unclear if
+  that is useful or not.\<close>
+lemma uminus_lit_of_nat:
+  \<open>- (literal_of_nat n) = (if even n then literal_of_nat (n+1) else literal_of_nat (n-1))\<close>
+  by (auto elim!: oddE)
+
+lemma literal_of_nat_literal_of_nat_eq[iff]: \<open>literal_of_nat x = literal_of_nat xa \<longleftrightarrow> x = xa\<close>
+  by auto presburger+
+
+definition nat_lit_rel :: \<open>(nat \<times> nat literal) set\<close> where
+  \<open>nat_lit_rel =  br literal_of_nat (\<lambda>_. True)\<close>
+
+abbreviation nat_lit_assn :: \<open>nat literal \<Rightarrow> nat \<Rightarrow> assn\<close> where
+  \<open>nat_lit_assn \<equiv> pure nat_lit_rel\<close>
+
+definition unat_lit_rel :: \<open>(uint32 \<times> nat literal) set\<close> where
+  \<open>unat_lit_rel \<equiv> uint32_nat_rel O nat_lit_rel\<close>
+
+abbreviation unat_lit_assn :: \<open>nat literal \<Rightarrow> uint32 \<Rightarrow> assn\<close> where
+  \<open>unat_lit_assn \<equiv> pure unat_lit_rel\<close>
+
+lemma hr_comp_uint32_nat_assn_nat_lit_rel[simp]:
+  \<open>hr_comp uint32_nat_assn nat_lit_rel = unat_lit_assn\<close>
+  by (auto simp: hrp_comp_def hr_comp_def uint32_nat_rel_def
+        hr_comp_pure br_def unat_lit_rel_def)
+
+fun pair_of_ann_lit :: \<open>('a, 'b) ann_lit \<Rightarrow> 'a literal \<times> 'b option\<close> where
+  \<open>pair_of_ann_lit (Propagated L D) = (L, Some D)\<close>
+| \<open>pair_of_ann_lit (Decided L) = (L, None)\<close>
+
+fun ann_lit_of_pair :: \<open>'a literal \<times> 'b option \<Rightarrow> ('a, 'b) ann_lit\<close> where
+  \<open>ann_lit_of_pair (L, Some D) = Propagated L D\<close>
+| \<open>ann_lit_of_pair (L, None) = Decided L\<close>
+
+lemma ann_lit_of_pair_alt_def:
+  \<open>ann_lit_of_pair (L, D) = (if D = None then Decided L else Propagated L (the D))\<close>
+  by (cases D) auto
+
+lemma ann_lit_of_pair_pair_of_ann_lit: \<open>ann_lit_of_pair (pair_of_ann_lit L) = L\<close>
+  by (cases L) auto
+
+lemma pair_of_ann_lit_ann_lit_of_pair: \<open>pair_of_ann_lit (ann_lit_of_pair L) = L\<close>
+  by (cases L; cases \<open>snd L\<close>) auto
+
+lemma literal_of_neq_eq_nat_of_lit_eq_iff: \<open>literal_of_nat b = L \<longleftrightarrow> b = nat_of_lit L\<close>
+  by (auto simp del: literal_of_nat.simps)
+
+lemma nat_of_lit_eq_iff[iff]: \<open>nat_of_lit xa = nat_of_lit x \<longleftrightarrow> x = xa\<close>
+  apply (cases x; cases xa) by auto presburger+
+
+lemma
+   nat_lit_rel_right_unique: \<open>IS_RIGHT_UNIQUE nat_lit_rel\<close> and
+   nat_lit_rel_left_unique: \<open>IS_LEFT_UNIQUE nat_lit_rel\<close>
+  unfolding single_valued_def nat_lit_rel_def IS_LEFT_UNIQUE_def
+  by (auto simp: br_def) presburger
+
+definition ann_lit_rel:: \<open>('a \<times> nat) set \<Rightarrow> ('b \<times> nat option) set \<Rightarrow>
+    (('a \<times> 'b) \<times> (nat, nat) ann_lit) set\<close> where
+  ann_lit_rel_internal_def:
+  \<open>ann_lit_rel R R' = {(a, b). \<exists>c d. (fst a, c) \<in> R \<and> (snd a, d) \<in> R' \<and>
+      b = ann_lit_of_pair (literal_of_nat c, d)}\<close>
+
+type_synonym ann_lit_wl = \<open>uint32 \<times> nat option\<close>
+type_synonym ann_lits_wl = \<open>ann_lit_wl list\<close>
+type_synonym ann_lit_wl_fast = \<open>uint32 \<times> uint32 option\<close>
+type_synonym ann_lits_wl_fast = \<open>ann_lit_wl_fast list\<close>
+
+definition nat_ann_lit_rel :: \<open>(ann_lit_wl \<times> (nat, nat) ann_lit) set\<close> where
+  nat_ann_lit_rel_internal_def: \<open>nat_ann_lit_rel = \<langle>uint32_nat_rel, \<langle>nat_rel\<rangle>option_rel\<rangle>ann_lit_rel\<close>
+
+lemma ann_lit_rel_def:
+  \<open>\<langle>R, R'\<rangle>ann_lit_rel = {(a, b). \<exists>c d. (fst a, c) \<in> R \<and> (snd a, d) \<in> R' \<and>
+      b = ann_lit_of_pair (literal_of_nat c, d)}\<close>
+  unfolding nat_ann_lit_rel_internal_def ann_lit_rel_internal_def relAPP_def ..
+
+lemma nat_ann_lit_rel_def:
+  \<open>nat_ann_lit_rel = {(a, b). b = ann_lit_of_pair ((\<lambda>(a,b). (literal_of_nat (nat_of_uint32 a), b)) a)}\<close>
+  unfolding nat_ann_lit_rel_internal_def ann_lit_rel_def
+  apply (auto simp: option_rel_def ex_disj_distrib uint32_nat_rel_def br_def)
+   apply (case_tac b)
+    apply auto
+   apply (case_tac b)
+   apply auto
+  done
+
+definition nat_ann_lits_rel :: \<open>(ann_lits_wl \<times> (nat, nat) ann_lits) set\<close> where
+  \<open>nat_ann_lits_rel = \<langle>nat_ann_lit_rel\<rangle>list_rel\<close>
+
+abbreviation pair_nat_ann_lit_assn :: \<open>(nat, nat) ann_lit \<Rightarrow> ann_lit_wl \<Rightarrow> assn\<close> where
+  \<open>pair_nat_ann_lit_assn \<equiv> pure nat_ann_lit_rel\<close>
+
+abbreviation pair_nat_ann_lits_assn :: \<open>(nat, nat) ann_lits \<Rightarrow> ann_lits_wl \<Rightarrow> assn\<close> where
+  \<open>pair_nat_ann_lits_assn \<equiv> list_assn pair_nat_ann_lit_assn\<close>
+
+abbreviation pair_nat_ann_lit_fast_assn :: \<open>(nat, nat) ann_lit \<Rightarrow> ann_lit_wl_fast \<Rightarrow> assn\<close> where
+  \<open>pair_nat_ann_lit_fast_assn \<equiv> hr_comp (uint32_assn *a option_assn uint32_nat_assn) nat_ann_lit_rel\<close>
+
+abbreviation pair_nat_ann_lits_fast_assn :: \<open>(nat, nat) ann_lits \<Rightarrow> ann_lits_wl_fast \<Rightarrow> assn\<close> where
+  \<open>pair_nat_ann_lits_fast_assn \<equiv> list_assn pair_nat_ann_lit_fast_assn\<close>
+
+lemma nat_ann_lits_rel_Cons[iff]:
+  \<open>(x # xs, y # ys) \<in> nat_ann_lits_rel \<longleftrightarrow> (x, y) \<in> nat_ann_lit_rel \<and> (xs, ys) \<in> nat_ann_lits_rel\<close>
+  by (auto simp: nat_ann_lits_rel_def)
+
+
+
+subsubsection \<open>Code\<close>
+
+lemma [sepref_fr_rules]: \<open>(return o id, RETURN o nat_of_lit) \<in> unat_lit_assn\<^sup>k \<rightarrow>\<^sub>a uint32_nat_assn\<close>
+  by sepref_to_hoare
+     (sep_auto simp: uint32_nat_rel_def br_def unat_lit_rel_def nat_lit_rel_def)
+
+definition (in -)the_is_empty where
+  \<open>the_is_empty D = Multiset.is_empty (the D)\<close>
+
+
+subsection \<open>Atoms with bound\<close>
+
+abbreviation uint_max :: nat where
+  \<open>uint_max \<equiv> uint32_max\<close>
+
+lemmas uint_max_def = uint32_max_def
+
+context isasat_input_ops
+begin
+
+abbreviation D\<^sub>0 :: \<open>(nat \<times> nat literal) set\<close> where
+  \<open>D\<^sub>0 \<equiv> (\<lambda>L. (nat_of_lit L, L)) ` set_mset \<L>\<^sub>a\<^sub>l\<^sub>l\<close>
+
+definition length_ll_f where
+  \<open>length_ll_f W L = length (W L)\<close>
+
+lemma length_ll_length_ll_f:
+  \<open>(uncurry (RETURN oo length_ll), uncurry (RETURN oo length_ll_f)) \<in>
+     [\<lambda>(W, L). L \<in># \<L>\<^sub>a\<^sub>l\<^sub>l]\<^sub>f ((\<langle>Id\<rangle>map_fun_rel D\<^sub>0) \<times>\<^sub>r nat_lit_rel) \<rightarrow>
+       \<langle>nat_rel\<rangle> nres_rel\<close>
+  unfolding length_ll_def length_ll_f_def
+  by (fastforce simp: fref_def map_fun_rel_def prod_rel_def nres_rel_def p2rel_def br_def
+      nat_lit_rel_def)
+
+abbreviation array_watched_assn
+  :: \<open>(nat literal \<Rightarrow> (nat \<times> nat literal \<times> bool) list) \<Rightarrow> ((nat \<times> uint32 \<times> bool) array_list) array \<Rightarrow>
+     assn\<close>
+where
+  \<open>array_watched_assn \<equiv> hr_comp (arrayO_assn (arl_assn (nat_assn *a unat_lit_assn *a bool_assn))) 
+    (\<langle>Id\<rangle>map_fun_rel D\<^sub>0)\<close>
+
+
+lemma ex_list_watched:
+  fixes W :: \<open>nat literal \<Rightarrow> 'a list\<close>
+  shows \<open>\<exists>aa. \<forall>x\<in>#\<L>\<^sub>a\<^sub>l\<^sub>l. nat_of_lit x < length aa \<and> aa ! nat_of_lit x = W x\<close>
+  (is \<open>\<exists>aa. ?P aa\<close>)
+proof -
+  define D' where \<open>D' = D\<^sub>0\<close>
+  define \<L>\<^sub>a\<^sub>l\<^sub>l' where \<open>\<L>\<^sub>a\<^sub>l\<^sub>l' = \<L>\<^sub>a\<^sub>l\<^sub>l\<close>
+  define D'' where \<open>D'' = mset_set (snd ` D')\<close>
+  let ?f = \<open>(\<lambda>L a. a[nat_of_lit L:= W L])\<close>
+  interpret comp_fun_commute ?f
+    apply standard
+    apply (case_tac \<open>y = x\<close>)
+     apply (solves simp)
+    apply (intro ext)
+    apply (subst (asm) lit_of_nat_nat_of_lit[symmetric])
+    apply (subst (asm)(3) lit_of_nat_nat_of_lit[symmetric])
+    apply (clarsimp simp only: comp_def intro!: list_update_swap)
+    done
+  define aa where
+    \<open>aa \<equiv> fold_mset ?f (replicate (1+Max (nat_of_lit ` snd ` D')) []) (mset_set (snd ` D'))\<close>
+  have length_fold: \<open>length (fold_mset (\<lambda>L a. a[nat_of_lit L := W L]) l M) = length l\<close> for l M
+    by (induction M) auto
+  have length_aa: \<open>length aa = Suc (Max (nat_of_lit ` snd ` D'))\<close>
+    unfolding aa_def D''_def[symmetric] by (simp add: length_fold)
+  have H: \<open>x \<in># \<L>\<^sub>a\<^sub>l\<^sub>l \<Longrightarrow>
+      length l \<ge> Suc (Max (nat_of_lit ` set_mset \<L>\<^sub>a\<^sub>l\<^sub>l)) \<Longrightarrow>
+      fold_mset (\<lambda>L a. a[nat_of_lit L := W L]) l (remdups_mset \<L>\<^sub>a\<^sub>l\<^sub>l) ! nat_of_lit x = W x\<close>
+    for x l
+    unfolding \<L>\<^sub>a\<^sub>l\<^sub>l'_def[symmetric]
+    apply (induction \<L>\<^sub>a\<^sub>l\<^sub>l' arbitrary: l)
+    subgoal by simp
+    subgoal for xa Ls l
+      apply (case_tac \<open>(nat_of_lit ` set_mset Ls) = {}\<close>)
+       apply (solves simp)
+      apply (auto simp: less_Suc_eq_le length_fold)
+      done
+    done
+  have H': \<open>aa ! nat_of_lit x = W x\<close> if \<open>x \<in># \<L>\<^sub>a\<^sub>l\<^sub>l\<close> for x
+    using that unfolding aa_def D'_def
+    by (auto simp: D'_def image_image remdups_mset_def[symmetric]
+        less_Suc_eq_le intro!: H)
+  have \<open>?P aa\<close>
+    by (auto simp: D'_def image_image remdups_mset_def[symmetric]
+        less_Suc_eq_le length_aa H')
+  then show ?thesis
+    by blast
+qed
+
+lemma length_aa_length_ll_f[sepref_fr_rules]:
+  \<open>(uncurry length_aa_u, uncurry (RETURN oo length_ll_f)) \<in>
+    [\<lambda>(W, L). L \<in># \<L>\<^sub>a\<^sub>l\<^sub>l]\<^sub>a
+      array_watched_assn\<^sup>k *\<^sub>a unat_lit_assn\<^sup>k \<rightarrow> nat_assn\<close>
+  (is \<open>?c \<in> [?pre]\<^sub>a ?im \<rightarrow> ?f\<close>)
+proof -
+  have P: \<open>is_pure nat_assn\<close>
+    by auto
+  have H: \<open>(uncurry length_aa_u, uncurry (RETURN \<circ>\<circ> length_ll_f))
+     \<in> [comp_PRE (\<langle>Id\<rangle>map_fun_rel D\<^sub>0 \<times>\<^sub>r nat_lit_rel)
+     (\<lambda>(W, L). L \<in># \<L>\<^sub>a\<^sub>l\<^sub>l) (\<lambda>_ (xs, i). i < length xs)
+     (\<lambda>_. True)]\<^sub>a hrp_comp
+                     ((arrayO_assn (arl_assn (nat_assn *a unat_lit_assn *a bool_assn)))\<^sup>k *\<^sub>a
+                      uint32_nat_assn\<^sup>k)
+                     (\<langle>Id\<rangle>map_fun_rel D\<^sub>0 \<times>\<^sub>r
+                      nat_lit_rel) \<rightarrow> hr_comp nat_assn nat_rel\<close>
+    (is \<open>_ \<in> [?pre']\<^sub>a ?im' \<rightarrow> ?f'\<close>)
+    using hfref_compI_PRE_aux[OF length_aa_u_hnr length_ll_length_ll_f] .
+
+  have 1: \<open>?pre' = ?pre\<close>
+    using ex_list_watched
+    by (fastforce simp: comp_PRE_def prod_rel_def_internal relAPP_def map_fun_rel_def[abs_def]
+        p2rel_def literal_of_neq_eq_nat_of_lit_eq_iff length_ll_def nat_lit_rel_def br_def
+        simp del: literal_of_nat.simps)
+
+  have 2: \<open>?im' = ?im\<close>
+    unfolding prod_hrp_comp by (auto simp: hrp_comp_def hr_comp_def)
+  have 3: \<open>?f' = ?f\<close>
+    by (auto simp: hrp_comp_def hr_comp_def)
+
+  show ?thesis
+    using H unfolding 1 2 3 .
+qed
+
+end
+
+
+locale isasat_input_bounded =
+  isasat_input_ops \<A>\<^sub>i\<^sub>n
+  for \<A>\<^sub>i\<^sub>n :: \<open>nat multiset\<close> +
+  assumes
+    in_\<L>\<^sub>a\<^sub>l\<^sub>l_less_uint_max: \<open>\<forall>L \<in># \<L>\<^sub>a\<^sub>l\<^sub>l. nat_of_lit L \<le> uint_max\<close>
+
+locale isasat_input_bounded_nempty =
+  isasat_input_bounded \<A>\<^sub>i\<^sub>n
+  for \<A>\<^sub>i\<^sub>n :: \<open>nat multiset\<close> +
+  assumes
+    \<A>\<^sub>i\<^sub>n_nempty: \<open>\<A>\<^sub>i\<^sub>n \<noteq> {#}\<close>
+
+
+context isasat_input_bounded
+begin
+
+lemma in_\<L>\<^sub>a\<^sub>l\<^sub>l_less_uint_max': \<open>L \<in># \<L>\<^sub>a\<^sub>l\<^sub>l \<Longrightarrow> nat_of_lit L \<le> uint_max\<close>
+  using in_\<L>\<^sub>a\<^sub>l\<^sub>l_less_uint_max by auto
+
+lemma in_\<A>\<^sub>i\<^sub>n_less_than_uint_max_div_2:
+  \<open>L \<in># \<A>\<^sub>i\<^sub>n \<Longrightarrow> L \<le> uint_max div 2\<close>
+  using in_\<L>\<^sub>a\<^sub>l\<^sub>l_less_uint_max'[of \<open>Neg L\<close>]
+  unfolding Ball_def atms_of_\<L>\<^sub>a\<^sub>l\<^sub>l_\<A>\<^sub>i\<^sub>n in_\<L>\<^sub>a\<^sub>l\<^sub>l_atm_of_in_atms_of_iff
+  by (auto simp: uint_max_def)
+
+lemma simple_clss_size_upper_div2':
+  assumes
+    lits: \<open>literals_are_in_\<L>\<^sub>i\<^sub>n C\<close> and
+    dist: \<open>distinct_mset C\<close> and
+    tauto: \<open>\<not>tautology C\<close> and
+    in_\<L>\<^sub>a\<^sub>l\<^sub>l_less_uint_max: \<open>\<forall>L \<in># \<L>\<^sub>a\<^sub>l\<^sub>l. nat_of_lit L < uint_max - 1\<close>
+  shows \<open>size C \<le> uint_max div 2\<close>
+proof -
+  let ?C = \<open>atm_of `# C\<close>
+  have \<open>distinct_mset ?C\<close>
+  proof (rule ccontr)
+    assume \<open>\<not> ?thesis\<close>
+    then obtain K where \<open>\<not>count (atm_of `# C) K \<le> Suc 0\<close>
+      unfolding distinct_mset_count_less_1
+      by auto
+    then have \<open>count (atm_of `# C) K \<ge> 2\<close>
+      by auto
+    then obtain L L' C' where
+      C: \<open>C = {#L, L'#} + C'\<close> and L_L': \<open>atm_of L = atm_of L'\<close>
+      by (auto dest!: count_image_mset_multi_member_split_2)
+    then show False
+      using dist tauto by (auto simp: atm_of_eq_atm_of tautology_add_mset)
+  qed
+  then have card: \<open>size ?C = card (set_mset ?C)\<close>
+    using distinct_mset_size_eq_card by blast
+  have size: \<open>size ?C = size C\<close>
+    using dist tauto
+    by (induction C) (auto simp: tautology_add_mset)
+  have m: \<open>set_mset ?C \<subseteq> {0..<uint_max div 2}\<close>
+  proof
+    fix L
+    assume \<open>L \<in> set_mset ?C\<close>
+    then have \<open>L \<in> atms_of \<L>\<^sub>a\<^sub>l\<^sub>l\<close>
+    using lits by (auto simp: literals_are_in_\<L>\<^sub>i\<^sub>n_def atm_of_lit_in_atms_of
+        in_all_lits_of_m_ain_atms_of_iff subset_iff)
+    then have \<open>Pos L \<in># \<L>\<^sub>a\<^sub>l\<^sub>l\<close>
+      using lits by (auto simp: in_\<L>\<^sub>a\<^sub>l\<^sub>l_atm_of_in_atms_of_iff)
+    then have \<open>nat_of_lit (Pos L) < uint_max - 1\<close>
+      using in_\<L>\<^sub>a\<^sub>l\<^sub>l_less_uint_max by (auto simp: atm_of_lit_in_atms_of
+        in_all_lits_of_m_ain_atms_of_iff subset_iff)
+    then have \<open>L < uint_max div 2\<close>
+       by (auto simp: atm_of_lit_in_atms_of
+        in_all_lits_of_m_ain_atms_of_iff subset_iff uint_max_def)
+    then show \<open>L \<in> {0..<uint_max div 2}\<close>
+       by (auto simp: atm_of_lit_in_atms_of uint_max_def
+        in_all_lits_of_m_ain_atms_of_iff subset_iff)
+  qed
+  moreover have \<open>card \<dots> =  uint_max div 2\<close>
+    by auto
+  ultimately have \<open>card (set_mset ?C) \<le> uint_max div 2\<close>
+    using card_mono[OF _ m] by auto
+  then show ?thesis
+    unfolding card[symmetric] size .
+qed
+
+
+lemma simple_clss_size_upper_div2:
+  assumes
+   lits: \<open>literals_are_in_\<L>\<^sub>i\<^sub>n C\<close> and
+   dist: \<open>distinct_mset C\<close> and
+   tauto: \<open>\<not>tautology C\<close>
+  shows \<open>size C \<le> 1 + uint_max div 2\<close>
+proof -
+  let ?C = \<open>atm_of `# C\<close>
+  have \<open>distinct_mset ?C\<close>
+  proof (rule ccontr)
+    assume \<open>\<not> ?thesis\<close>
+    then obtain K where \<open>\<not>count (atm_of `# C) K \<le> Suc 0\<close>
+      unfolding distinct_mset_count_less_1
+      by auto
+    then have \<open>count (atm_of `# C) K \<ge> 2\<close>
+      by auto
+    then obtain L L' C' where
+      C: \<open>C = {#L, L'#} + C'\<close> and L_L': \<open>atm_of L = atm_of L'\<close>
+      by (auto dest!: count_image_mset_multi_member_split_2)
+    then show False
+      using dist tauto by (auto simp: atm_of_eq_atm_of tautology_add_mset)
+  qed
+  then have card: \<open>size ?C = card (set_mset ?C)\<close>
+    using distinct_mset_size_eq_card by blast
+  have size: \<open>size ?C = size C\<close>
+    using dist tauto
+    by (induction C) (auto simp: tautology_add_mset)
+  have m: \<open>set_mset ?C \<subseteq> {0..uint_max div 2}\<close>
+  proof
+    fix L
+    assume \<open>L \<in> set_mset ?C\<close>
+    then have \<open>L \<in> atms_of \<L>\<^sub>a\<^sub>l\<^sub>l\<close>
+    using lits by (auto simp: literals_are_in_\<L>\<^sub>i\<^sub>n_def atm_of_lit_in_atms_of
+        in_all_lits_of_m_ain_atms_of_iff subset_iff)
+    then have \<open>Pos L \<in># \<L>\<^sub>a\<^sub>l\<^sub>l\<close>
+      using lits by (auto simp: in_\<L>\<^sub>a\<^sub>l\<^sub>l_atm_of_in_atms_of_iff)
+    then have \<open>nat_of_lit (Pos L) \<le> uint_max\<close>
+      using in_\<L>\<^sub>a\<^sub>l\<^sub>l_less_uint_max by (auto simp: atm_of_lit_in_atms_of
+        in_all_lits_of_m_ain_atms_of_iff subset_iff)
+    then have \<open>L \<le> uint_max div 2\<close>
+       by (auto simp: atm_of_lit_in_atms_of
+        in_all_lits_of_m_ain_atms_of_iff subset_iff uint_max_def)
+    then show \<open>L \<in> {0 .. uint_max div 2}\<close>
+       by (auto simp: atm_of_lit_in_atms_of uint_max_def
+        in_all_lits_of_m_ain_atms_of_iff subset_iff)
+  qed
+  moreover have \<open>card \<dots> =  1 + uint_max div 2\<close>
+    by auto
+  ultimately have \<open>card (set_mset ?C) \<le> 1 + uint_max div 2\<close>
+    using card_mono[OF _ m] by auto
+  then show ?thesis
+    unfolding card[symmetric] size .
+qed
+
+lemma clss_size_uint_max:
+  assumes
+   lits: \<open>literals_are_in_\<L>\<^sub>i\<^sub>n C\<close> and
+   dist: \<open>distinct_mset C\<close>
+  shows \<open>size C \<le> uint_max + 2\<close>
+proof -
+  let ?posC = \<open>filter_mset is_pos C\<close>
+  let ?negC = \<open>filter_mset is_neg C\<close>
+  have C: \<open>C = ?posC + ?negC\<close>
+    apply (subst multiset_partition[of _ is_pos])
+    by auto
+  have \<open>literals_are_in_\<L>\<^sub>i\<^sub>n ?posC\<close>
+    by (rule literals_are_in_\<L>\<^sub>i\<^sub>n_mono[OF lits]) auto
+  moreover have \<open>distinct_mset ?posC\<close>
+    by (rule distinct_mset_mono[OF _dist]) auto
+  ultimately have pos: \<open>size ?posC \<le> 1 + uint_max div 2\<close>
+    by (rule simple_clss_size_upper_div2) (auto simp: tautology_decomp)
+
+  have \<open>literals_are_in_\<L>\<^sub>i\<^sub>n ?negC\<close>
+    by (rule literals_are_in_\<L>\<^sub>i\<^sub>n_mono[OF lits]) auto
+  moreover have \<open>distinct_mset ?negC\<close>
+    by (rule distinct_mset_mono[OF _dist]) auto
+  ultimately have neg: \<open>size ?negC \<le> 1 + uint_max div 2\<close>
+    by (rule simple_clss_size_upper_div2) (auto simp: tautology_decomp)
+
+  show ?thesis
+    apply (subst C)
+    apply (subst size_union)
+    using pos neg by linarith
+qed
+
+lemma clss_size_uint64_max:
+  assumes
+   lits: \<open>literals_are_in_\<L>\<^sub>i\<^sub>n C\<close> and
+   dist: \<open>distinct_mset C\<close>
+ shows \<open>size C < uint64_max\<close>
+  using clss_size_uint_max[OF assms] by (auto simp: uint32_max_def uint64_max_def)
+
+lemma clss_size_upper:
+  assumes
+   lits: \<open>literals_are_in_\<L>\<^sub>i\<^sub>n C\<close> and
+   dist: \<open>distinct_mset C\<close> and
+   in_\<L>\<^sub>a\<^sub>l\<^sub>l_less_uint_max: \<open>\<forall>L \<in># \<L>\<^sub>a\<^sub>l\<^sub>l. nat_of_lit L < uint_max - 1\<close>
+ shows \<open>size C \<le> uint_max\<close>
+proof -
+  let ?A = \<open>remdups_mset (atm_of `# C)\<close>
+  have [simp]: \<open>distinct_mset (poss ?A)\<close> \<open>distinct_mset (negs ?A)\<close>
+    by (simp_all add: distinct_image_mset_inj inj_on_def)
+
+  have \<open>C \<subseteq># poss ?A + negs ?A\<close>
+    apply (rule distinct_subseteq_iff[THEN iffD1])
+    subgoal by (auto simp: dist distinct_mset_add disjunct_not_in)
+    subgoal by (auto simp: dist distinct_mset_add disjunct_not_in)
+    subgoal
+      apply rule
+      using literal.exhaust_sel by (auto simp: image_iff)
+    done
+  have [simp]: \<open>literals_are_in_\<L>\<^sub>i\<^sub>n (poss ?A)\<close> \<open>literals_are_in_\<L>\<^sub>i\<^sub>n (negs ?A)\<close>
+    using lits
+    by (auto simp: literals_are_in_\<L>\<^sub>i\<^sub>n_negs_remdups_mset literals_are_in_\<L>\<^sub>i\<^sub>n_poss_remdups_mset)
+
+  have \<open>\<not> tautology (poss ?A)\<close> \<open>\<not> tautology (negs ?A)\<close>
+    by (auto simp: tautology_decomp)
+  then have \<open>size (poss ?A) \<le> uint_max div 2\<close> and \<open>size (negs ?A) \<le> uint_max div 2\<close>
+    using simple_clss_size_upper_div2'[of \<open>poss ?A\<close>]
+      simple_clss_size_upper_div2'[of \<open>negs ?A\<close>] in_\<L>\<^sub>a\<^sub>l\<^sub>l_less_uint_max
+    by auto
+  then have \<open>size C \<le> uint_max div 2 + uint_max div 2\<close>
+    using \<open>C \<subseteq># poss (remdups_mset (atm_of `# C)) + negs (remdups_mset (atm_of `# C))\<close>
+      size_mset_mono by fastforce
+  then show ?thesis by (auto simp: uint_max_def)
+qed
+
+lemma (in isasat_input_bounded)
+  assumes
+    lits: \<open>literals_are_in_\<L>\<^sub>i\<^sub>n_trail M\<close> and
+    n_d: \<open>no_dup M\<close>
+  shows
+    literals_are_in_\<L>\<^sub>i\<^sub>n_trail_length_le_uint32_max:
+      \<open>length M \<le> Suc (uint_max div 2)\<close> and
+    literals_are_in_\<L>\<^sub>i\<^sub>n_trail_count_decided_uint_max:
+      \<open>count_decided M \<le> Suc (uint_max div 2)\<close> and
+    literals_are_in_\<L>\<^sub>i\<^sub>n_trail_get_level_uint_max:
+      \<open>get_level M L \<le> Suc (uint_max div 2)\<close>
+proof -
+  have \<open>length M = card (atm_of ` lits_of_l M)\<close>
+    using no_dup_length_eq_card_atm_of_lits_of_l[OF n_d] .
+  moreover have \<open>atm_of ` lits_of_l M \<subseteq> set_mset \<A>\<^sub>i\<^sub>n\<close>
+    using lits unfolding literals_are_in_\<L>\<^sub>i\<^sub>n_trail_atm_of by auto
+  ultimately have \<open>length M \<le> card (set_mset \<A>\<^sub>i\<^sub>n)\<close>
+    by (simp add: card_mono)
+  moreover {
+    have \<open>set_mset \<A>\<^sub>i\<^sub>n \<subseteq> {0 ..< (uint_max div 2) + 1}\<close>
+      using in_\<A>\<^sub>i\<^sub>n_less_than_uint_max_div_2 by (fastforce simp: in_\<L>\<^sub>a\<^sub>l\<^sub>l_atm_of_in_atms_of_iff
+          Ball_def atms_of_\<L>\<^sub>a\<^sub>l\<^sub>l_\<A>\<^sub>i\<^sub>n uint_max_def)
+    from subset_eq_atLeast0_lessThan_card[OF this] have \<open>card (set_mset \<A>\<^sub>i\<^sub>n) \<le> uint_max div 2 + 1\<close>
+      .
+  }
+  ultimately show \<open>length M \<le> Suc (uint_max div 2)\<close>
+    by linarith
+  moreover have \<open>count_decided M \<le> length M\<close>
+    unfolding count_decided_def by auto
+  ultimately show \<open>count_decided M \<le> Suc (uint_max div 2)\<close> by simp
+  then show \<open>get_level M L \<le> Suc (uint_max div 2)\<close>
+    using count_decided_ge_get_level[of M L]
+    by simp
+qed
+
+lemma length_trail_uint_max_div2:
+  assumes
+    M_\<L>\<^sub>a\<^sub>l\<^sub>l: \<open>\<forall>L\<in>set M. lit_of L \<in># \<L>\<^sub>a\<^sub>l\<^sub>l\<close> and n_d: \<open>no_dup M\<close>
+  shows \<open>length M \<le> uint_max div 2 + 1\<close>
+proof -
+  have dist_atm_M: \<open>distinct_mset {#atm_of (lit_of x). x \<in># mset M#}\<close>
+    using n_d by (metis distinct_mset_mset_distinct mset_map no_dup_def)
+  have incl: \<open>atm_of `# lit_of `# mset M \<subseteq># remdups_mset (atm_of `# \<L>\<^sub>a\<^sub>l\<^sub>l)\<close>
+    apply (subst distinct_subseteq_iff[THEN iffD1])
+    using assms dist_atm_M
+    by (auto simp: Decided_Propagated_in_iff_in_lits_of_l lits_of_def no_dup_distinct
+        atm_of_eq_atm_of)
+
+  have inj_on: \<open>inj_on nat_of_lit (set_mset (remdups_mset \<L>\<^sub>a\<^sub>l\<^sub>l))\<close>
+    by (auto simp: inj_on_def)
+  have H: \<open>xa \<in># \<L>\<^sub>a\<^sub>l\<^sub>l \<Longrightarrow> atm_of xa \<le> uint_max div 2\<close> for xa
+    using in_\<L>\<^sub>a\<^sub>l\<^sub>l_less_uint_max
+    by (cases xa) (auto simp: uint_max_def)
+  have \<open>remdups_mset (atm_of `# \<L>\<^sub>a\<^sub>l\<^sub>l) \<subseteq># mset [0..< 1 + (uint_max div 2)]\<close>
+    apply (subst distinct_subseteq_iff[THEN iffD1])
+    using H distinct_image_mset_inj[OF inj_on]
+    by (force simp del: literal_of_nat.simps simp: distinct_mset_mset_set
+        dest: le_neq_implies_less)+
+  note _ = size_mset_mono[OF this]
+  moreover have \<open>size (nat_of_lit `# remdups_mset \<L>\<^sub>a\<^sub>l\<^sub>l) = size (remdups_mset \<L>\<^sub>a\<^sub>l\<^sub>l)\<close>
+    by simp
+  ultimately have 2: \<open>size (remdups_mset (atm_of `# \<L>\<^sub>a\<^sub>l\<^sub>l)) \<le> 1 + uint_max div 2\<close>
+    by auto
+  from size_mset_mono[OF incl] have 1: \<open>length M \<le> size (remdups_mset (atm_of `# \<L>\<^sub>a\<^sub>l\<^sub>l))\<close>
+    unfolding uint_max_def count_decided_def
+    by (auto simp del: length_filter_le)
+  with 2 show ?thesis
+    by (auto simp: uint32_max_def)
+qed
+
+end
+
 text \<open>
   First we instantiate our types with sort heap and default, to have compatibility with code
   generation. The idea is simplify to create injections into the components of our datatypes.
@@ -105,7 +672,7 @@ lemma propagated_hnr[sepref_fr_rules]:
   \<open>(uncurry (return oo propagated), uncurry (RETURN oo Propagated)) \<in>
      unat_lit_assn\<^sup>k *\<^sub>a nat_assn\<^sup>k \<rightarrow>\<^sub>a pair_nat_ann_lit_assn\<close>
   by sepref_to_hoare (sep_auto simp: nat_ann_lit_rel_def propagated_def case_prod_beta p2rel_def
-      lit_of_natP_def br_def uint32_nat_rel_def unat_lit_rel_def nat_lit_rel_def
+      br_def uint32_nat_rel_def unat_lit_rel_def nat_lit_rel_def
       split: option.splits)
 
 definition decided where
@@ -115,7 +682,7 @@ lemma decided_hnr[sepref_fr_rules]:
   \<open>(return o decided, RETURN o Decided) \<in>
      unat_lit_assn\<^sup>k \<rightarrow>\<^sub>a pair_nat_ann_lit_assn\<close>
   by sepref_to_hoare (sep_auto simp: nat_ann_lit_rel_def decided_def case_prod_beta p2rel_def
-      lit_of_natP_def br_def uint32_nat_rel_def unat_lit_rel_def nat_lit_rel_def
+      br_def uint32_nat_rel_def unat_lit_rel_def nat_lit_rel_def
       split: option.splits)
 
 definition uminus_lit_imp :: \<open>nat \<Rightarrow> nat\<close> where
@@ -126,7 +693,7 @@ lemma uminus_lit_imp_uminus:
      nat_lit_rel \<rightarrow>\<^sub>f \<langle>nat_lit_rel\<rangle>nres_rel\<close>
   unfolding bitXOR_1_if_mod_2 uminus_lit_imp_def
   by (intro frefI nres_relI) (auto simp: nat_ann_lit_rel_def uminus_lit_imp_def case_prod_beta p2rel_def
-      lit_of_natP_def nat_lit_rel_def split: option.splits, presburger)
+      br_def nat_lit_rel_def split: option.splits, presburger)
 
 definition uminus_code :: \<open>uint32 \<Rightarrow> uint32\<close> where
   \<open>uminus_code L = bitXOR L 1\<close>
@@ -162,7 +729,7 @@ proof -
     unfolding bitXOR_1_if_mod_2 uminus_lit_imp_def
     apply sepref_to_hoare
     apply (sep_auto simp: nat_ann_lit_rel_def uminus_lit_imp_def case_prod_beta p2rel_def
-        lit_of_natP_def uint32_nat_rel_def br_def nat_of_uint32_XOR bitXOR_1_if_mod_2
+        uint32_nat_rel_def br_def nat_of_uint32_XOR bitXOR_1_if_mod_2
         split: option.splits)
     using One_nat_def bitXOR_1_if_mod_2 by presburger
   show ?thesis
@@ -248,13 +815,13 @@ definition atm_of_code :: \<open>uint32 \<Rightarrow> uint32\<close> where
 
 lemma atm_of_hnr[sepref_fr_rules]:
   \<open>(return o atm_of_code, RETURN o op_atm_of) \<in> unat_lit_assn\<^sup>k \<rightarrow>\<^sub>a uint32_nat_assn\<close>
-  by sepref_to_hoare (sep_auto simp: p2rel_def lit_of_natP_def uint32_nat_rel_def br_def
+  by sepref_to_hoare (sep_auto simp: p2rel_def uint32_nat_rel_def br_def
       Collect_eq_comp unat_lit_rel_def nat_of_uint32_shiftr nat_lit_rel_def atm_of_code_def)
 
 lemma lit_of_hnr[sepref_fr_rules]:
   \<open>(return o fst, RETURN o op_lit_of) \<in> pair_nat_ann_lit_assn\<^sup>k \<rightarrow>\<^sub>a unat_lit_assn\<close>
   by sepref_to_hoare
-    (sep_auto simp: p2rel_def nat_ann_lit_rel_def lit_of_natP_def uint32_nat_rel_def
+    (sep_auto simp: p2rel_def nat_ann_lit_rel_def uint32_nat_rel_def
       Collect_eq_comp br_def unat_lit_rel_def nat_lit_rel_def ann_lit_of_pair_alt_def
       split: if_splits)
 
@@ -262,7 +829,7 @@ lemma lit_of_fast_hnr[sepref_fr_rules]:
   \<open>(return o fst, RETURN o op_lit_of) \<in> pair_nat_ann_lit_fast_assn\<^sup>k \<rightarrow>\<^sub>a unat_lit_assn\<close>
   apply sepref_to_hoare
   apply (sep_auto simp: unat_lit_rel_def uint32_nat_rel_def)
-  apply (sep_auto simp: p2rel_def nat_ann_lit_rel_def lit_of_natP_def uint32_nat_rel_def
+  apply (sep_auto simp: p2rel_def nat_ann_lit_rel_def uint32_nat_rel_def
       Collect_eq_comp br_def unat_lit_rel_def nat_lit_rel_def ann_lit_of_pair_alt_def
       hr_comp_def prod.splits case_prod_beta
       split: if_splits)
@@ -278,7 +845,7 @@ proof -
     by presburger
   show ?thesis
     by sepref_to_hoare
-       (sep_auto simp: p2rel_def nat_ann_lit_rel_def lit_of_natP_def nat_lit_rel_def
+       (sep_auto simp: p2rel_def nat_ann_lit_rel_def nat_lit_rel_def
         br_def Collect_eq_comp uint32_nat_rel_def dvd_div_eq_iff unat_lit_rel_def
       split: if_splits)+
 qed
@@ -300,7 +867,7 @@ lemma in_nat_list_rel_list_all2_in_set_iff:
     apply (rotate_tac 2)
     apply (induction b ba rule: list_induct2)
      apply (solves simp)
-    apply (auto simp: p2rel_def lit_of_natP_same_leftD lit_of_natP_same_rightD nat_lit_rel_def)[]
+    apply (auto simp: p2rel_def nat_lit_rel_def br_def, presburger)[]
     done
   subgoal using list_all2_lengthD by auto
   done
@@ -365,7 +932,7 @@ lemma
   nat_lit_assn_left_unique:
     \<open>CONSTRAINT (IS_PURE IS_LEFT_UNIQUE) nat_lit_assn\<close>
    by (auto simp: IS_PURE_def single_valued_def p2rel_def IS_LEFT_UNIQUE_def nat_lit_rel_def
-      dest: lit_of_natP_same_rightD lit_of_natP_same_leftD)
+      br_def, presburger)
 
 definition find_decomp_wl_imp :: \<open>(nat, nat) ann_lits \<Rightarrow> nat clause \<Rightarrow> nat literal \<Rightarrow> (nat, nat) ann_lits nres\<close> where
   \<open>find_decomp_wl_imp = (\<lambda>M\<^sub>0 D L. do {
@@ -437,10 +1004,16 @@ definition (in -) find_decomp_wl_imp' :: \<open>(nat, nat) ann_lits \<Rightarrow
 
 lemma nth_ll_watched_app:
   \<open>(uncurry2 (RETURN ooo nth_rll), uncurry2 (RETURN ooo watched_app)) \<in>
-     [\<lambda>((W, L), i). L \<in># \<L>\<^sub>a\<^sub>l\<^sub>l]\<^sub>f ((\<langle>Id\<rangle>map_fun_rel D\<^sub>0) \<times>\<^sub>r p2rel lit_of_natP) \<times>\<^sub>r nat_rel \<rightarrow>
+     [\<lambda>((W, L), i). L \<in># \<L>\<^sub>a\<^sub>l\<^sub>l]\<^sub>f ((\<langle>Id\<rangle>map_fun_rel D\<^sub>0) \<times>\<^sub>r nat_lit_rel) \<times>\<^sub>r nat_rel \<rightarrow>
        \<langle>nat_rel \<times>\<^sub>r Id\<rangle> nres_rel\<close>
   unfolding watched_app_def nth_rll_def
-  by (fastforce simp: fref_def map_fun_rel_def prod_rel_def nres_rel_def p2rel_def lit_of_natP_def)
+  by (fastforce simp: fref_def map_fun_rel_def prod_rel_def nres_rel_def p2rel_def br_def
+      nat_lit_rel_def)
+
+lemma ex_literal_of_nat: \<open>\<exists>bb. b = literal_of_nat bb\<close>
+  by (cases b)
+    (auto simp: nat_of_lit_def split: if_splits; presburger; fail)+
+
 
 lemma nth_aa_watched_app[sepref_fr_rules]:
   \<open>(uncurry2 nth_aa_u, uncurry2 (RETURN ooo op_watched_app)) \<in>
@@ -452,24 +1025,24 @@ proof -
     by auto
   have H: \<open>(uncurry2 nth_aa_u, uncurry2 (RETURN \<circ>\<circ>\<circ> watched_app))
   \<in> [comp_PRE
-       (\<langle>Id\<rangle>map_fun_rel D\<^sub>0 \<times>\<^sub>f p2rel lit_of_natP \<times>\<^sub>f nat_rel)
+       (\<langle>Id\<rangle>map_fun_rel D\<^sub>0 \<times>\<^sub>f nat_lit_rel \<times>\<^sub>f nat_rel)
        (\<lambda>((W, L), i). L \<in># \<L>\<^sub>a\<^sub>l\<^sub>l)
        (\<lambda>_ ((x, L), L'). L < length x \<and> L' < length (x ! L))
        (\<lambda>_. True)]\<^sub>a
     hrp_comp ((arrayO_assn (arl_assn (nat_assn *a unat_lit_assn *a bool_assn)))\<^sup>k *\<^sub>a uint32_nat_assn\<^sup>k *\<^sub>a
                         nat_assn\<^sup>k)
               (\<langle>Id\<rangle>map_fun_rel D\<^sub>0 \<times>\<^sub>f
-                        p2rel lit_of_natP \<times>\<^sub>f
+                        nat_lit_rel \<times>\<^sub>f
                         nat_rel) \<rightarrow> hr_comp (nat_assn *a unat_lit_assn *a bool_assn) (nat_rel \<times>\<^sub>f Id)\<close>
     (is \<open>_ \<in> [?pre']\<^sub>a ?im' \<rightarrow> ?f'\<close>)
     using hfref_compI_PRE_aux[OF nth_aa_uint_hnr nth_ll_watched_app, OF P]
      .
 
   have 1: \<open>?pre' = ?pre\<close>
-    using ex_list_watched
-    by (fastforce simp: comp_PRE_def prod_rel_def_internal relAPP_def map_fun_rel_def[abs_def]
-        p2rel_def lit_of_natP_def literal_of_neq_eq_nat_of_lit_eq_iff length_ll_def
-        simp del: literal_of_nat.simps intro!: ext)
+    using ex_list_watched ex_literal_of_nat
+    by (auto simp: comp_PRE_def prod_rel_def_internal relAPP_def map_fun_rel_def[abs_def]
+        p2rel_def literal_of_neq_eq_nat_of_lit_eq_iff length_ll_def nat_lit_rel_def br_def
+        simp del: literal_of_nat.simps intro!: ext) fastforce
 
   have 2: \<open>?im' = ?im\<close>
     unfolding prod_hrp_comp by (auto simp: hrp_comp_def hr_comp_def nat_lit_rel_def p2rel_def
@@ -489,11 +1062,11 @@ lemma (in -) is_pos_hnr[sepref_fr_rules]:
 proof -
   have 1: \<open>(RETURN o (\<lambda>L. bitAND L 1 = 0), RETURN o is_pos) \<in> nat_lit_rel \<rightarrow>\<^sub>f \<langle>bool_rel\<rangle>nres_rel\<close>
     unfolding bitAND_1_mod_2 is_pos_code_def
-    by (intro nres_relI frefI) (auto simp: nat_lit_rel_def lit_of_natP_def split: if_splits)
+    by (intro nres_relI frefI) (auto simp: nat_lit_rel_def br_def split: if_splits, presburger)
   have 2: \<open>(return o is_pos_code, RETURN o (\<lambda>L. bitAND L 1 = 0)) \<in> uint32_nat_assn\<^sup>k \<rightarrow>\<^sub>a bool_assn\<close>
     apply sepref_to_hoare
     using nat_of_uint32_ao[of _ 1]
-    by (sep_auto simp: p2rel_def lit_of_natP_def unat_lit_rel_def uint32_nat_rel_def
+    by (sep_auto simp: p2rel_def unat_lit_rel_def uint32_nat_rel_def
         nat_lit_rel_def br_def nat_of_uint32_012 is_pos_code_def
         nat_of_uint32_0_iff nat_0_AND uint32_0_AND
         split: if_splits)+
@@ -513,7 +1086,7 @@ lemma delete_index_and_swap_ll_delete_index_and_swap_update:
   \<in>[\<lambda>((W, L), i). L \<in># \<L>\<^sub>a\<^sub>l\<^sub>l]\<^sub>f (\<langle>Id\<rangle>map_fun_rel D\<^sub>0 \<times>\<^sub>r nat_lit_rel) \<times>\<^sub>r nat_rel \<rightarrow>
       \<langle>\<langle>Id\<rangle>map_fun_rel D\<^sub>0\<rangle>nres_rel\<close>
   by (auto simp: delete_index_and_swap_ll_def uncurry_def fref_def nres_rel_def
-      delete_index_and_swap_update_def map_fun_rel_def p2rel_def lit_of_natP_def
+      delete_index_and_swap_update_def map_fun_rel_def p2rel_def nat_lit_rel_def br_def
       nth_list_update' nat_lit_rel_def
       simp del: literal_of_nat.simps)
 
@@ -533,8 +1106,8 @@ proof -
     using hfref_compI_PRE[OF delete_index_and_swap_aa_ll_hnr_u
         delete_index_and_swap_ll_delete_index_and_swap_update, of "nat_assn *a unat_lit_assn *a bool_assn"] by simp
   have b: \<open>\<exists>bb. (bb, b) \<in> nat_lit_rel\<close> for b
-    apply (auto simp: p2rel_def lit_of_natP_def Pos_div2_iff Neg_div2_iff nat_lit_rel_def)
-    using even_Suc by blast
+    using ex_literal_of_nat
+    by (auto simp: p2rel_def Pos_div2_iff Neg_div2_iff nat_lit_rel_def br_def)
   have ba_length_a_b: \<open>ba < length (a b)\<close>
     if bN: \<open>b \<in># \<L>\<^sub>a\<^sub>l\<^sub>l\<close> and
       H: \<open>\<And>aa bb. (\<forall>x\<in>#\<L>\<^sub>a\<^sub>l\<^sub>l. nat_of_lit x < length aa \<and> aa ! nat_of_lit x = a x) \<and>
@@ -552,16 +1125,16 @@ proof -
     obtain bb where bb: \<open>(bb, b) \<in> nat_lit_rel\<close>
       using b[of b] by blast
     show ?thesis
-      using H[of aa bb] aa bb aa_b_a_b by (auto simp: p2rel_def lit_of_natP_def nat_lit_rel_def)
+      using H[of aa bb] aa bb aa_b_a_b by (auto simp: p2rel_def nat_lit_rel_def br_def)
   qed
 
   have pre: \<open>?pre' = ?pre\<close>
   using ex_list_watched
-    apply (auto simp: comp_PRE_def map_fun_rel_def lit_of_natP_def
+    apply (auto simp: comp_PRE_def map_fun_rel_def nat_lit_rel_def br_def
         image_image ba_length_a_b
         Pos_div2_iff Neg_div2_iff all_conj_distrib length_ll_def
         intro!: ext split: if_splits)
-    apply (auto simp: p2rel_def nat_lit_rel_def lit_of_natP_def split: if_splits)
+    apply (auto simp: p2rel_def nat_lit_rel_def split: if_splits)
     by (metis atm_of_lit_of_nat ex_list_watched
       lit_of_nat_nat_of_lit literal_of_nat.simps)
 
@@ -586,7 +1159,7 @@ lemma append_ll_append_update:
   \<in>  [\<lambda>((W, L), i). L \<in># \<L>\<^sub>a\<^sub>l\<^sub>l]\<^sub>f
      \<langle>Id\<rangle>map_fun_rel D\<^sub>0 \<times>\<^sub>f unat_lit_rel \<times>\<^sub>f Id \<rightarrow> \<langle>\<langle>Id\<rangle>map_fun_rel D\<^sub>0\<rangle>nres_rel\<close>
   by (auto simp: append_ll_def uncurry_def fref_def nres_rel_def
-      delete_index_and_swap_update_def map_fun_rel_def p2rel_def lit_of_natP_def
+      delete_index_and_swap_update_def map_fun_rel_def p2rel_def nat_lit_rel_def
       nth_list_update' append_update_def nat_lit_rel_def unat_lit_rel_def br_def
       uint32_nat_rel_def
       simp del: literal_of_nat.simps)
@@ -618,14 +1191,14 @@ proof -
         append_ll_append_update, of \<open>(nat_assn *a unat_lit_assn *a bool_assn)\<close>]
     unfolding append_el_aa_append_el_aa_u' by simp
   have b: \<open>\<exists>bb. (bb, b) \<in> nat_lit_rel\<close> for b
-    apply (auto simp: p2rel_def lit_of_natP_def Pos_div2_iff Neg_div2_iff nat_lit_rel_def)
-    using even_Suc by blast
+    using ex_literal_of_nat
+    by (auto simp: p2rel_def Pos_div2_iff Neg_div2_iff nat_lit_rel_def br_def)
 
   have pre: \<open>?pre' = ?pre\<close>
-    apply (auto simp: comp_PRE_def map_fun_rel_def lit_of_natP_def image_image
+    apply (auto simp: comp_PRE_def map_fun_rel_def image_image
         Pos_div2_iff Neg_div2_iff all_conj_distrib length_ll_def
         intro!: ext split: if_splits)
-    by (auto simp: p2rel_def lit_of_natP_def unat_lit_rel_def br_def nat_lit_rel_def uint32_nat_rel_def
+    by (auto simp: p2rel_def unat_lit_rel_def br_def nat_lit_rel_def uint32_nat_rel_def
         split: if_splits)
 
   have
@@ -671,7 +1244,7 @@ lemma lit_and_ann_of_propagated_hnr[sepref_fr_rules]:
   apply sepref_to_hoare
   apply (rename_tac x x')
   apply (case_tac x)
-  by (sep_auto simp: nat_ann_lit_rel_def p2rel_def lit_of_natP_def
+  by (sep_auto simp: nat_ann_lit_rel_def p2rel_def nat_lit_rel_def
       Propagated_eq_ann_lit_of_pair_iff unat_lit_rel_def uint32_nat_rel_def Collect_eq_comp
       br_def Collect_eq_comp nat_lit_rel_def
       simp del: literal_of_nat.simps)+
@@ -734,6 +1307,29 @@ proof -
     done
 qed
 
+
+lemma Pos_unat_lit_assn:
+  \<open>(return o (\<lambda>n. two_uint32 * n), RETURN o Pos) \<in> [\<lambda>L. Pos L \<in># \<L>\<^sub>a\<^sub>l\<^sub>l]\<^sub>a uint32_nat_assn\<^sup>k \<rightarrow>
+     unat_lit_assn\<close>
+  apply sepref_to_hoare
+  using in_\<L>\<^sub>a\<^sub>l\<^sub>l_less_uint_max
+  by (sep_auto simp: unat_lit_rel_def nat_lit_rel_def uint32_nat_rel_def br_def Collect_eq_comp
+      nat_of_uint32_distrib_mult2)
+
+lemma Neg_unat_lit_assn:
+  \<open>(return o (\<lambda>n. two_uint32 * n +1), RETURN o Neg) \<in> [\<lambda>L. Pos L \<in># \<L>\<^sub>a\<^sub>l\<^sub>l]\<^sub>a uint32_nat_assn\<^sup>k \<rightarrow>
+      unat_lit_assn\<close>
+  apply sepref_to_hoare
+  using in_\<L>\<^sub>a\<^sub>l\<^sub>l_less_uint_max
+  by (sep_auto simp: unat_lit_rel_def nat_lit_rel_def uint32_nat_rel_def br_def Collect_eq_comp
+      nat_of_uint32_distrib_mult2_plus1 uint_max_def)
 end
+
+lemma Pos_unat_lit_assn':
+  \<open>(return o (\<lambda>n. two_uint32 * n), RETURN o Pos) \<in> [\<lambda>L. L \<le> uint_max div 2]\<^sub>a uint32_nat_assn\<^sup>k \<rightarrow>
+     unat_lit_assn\<close>
+  apply sepref_to_hoare
+  by (sep_auto simp: unat_lit_rel_def nat_lit_rel_def uint32_nat_rel_def br_def Collect_eq_comp
+      nat_of_uint32_distrib_mult2 uint_max_def)
 
 end
