Weidenbach_Book/IsaSAT_Arena.thy
@@ -1,5 +1,5 @@
 theory IsaSAT_Arena
-imports Watched_Literals.Watched_Literals_Watch_List_Code_Common
+imports IsaSAT_Literals
   Watched_Literals.WB_More_Refinement_List
 begin
 
